Weidenbach_Book/Watched_Literals_Watch_List_Initialisation.thy
@@ -5,95 +5,200 @@ begin
 
 subsection \<open>Initialisation\<close>
 
-fun calculate_correct_watching
-  :: \<open>'v clauses_l \<Rightarrow> ('v literal \<Rightarrow> watched) \<Rightarrow> nat \<Rightarrow> ('v literal \<Rightarrow> watched)\<close> where
-  \<open>calculate_correct_watching [] W _ = W\<close>
-| \<open>calculate_correct_watching (C # N) W i =
-     (let W = calculate_correct_watching N W (Suc i) in
-     if C = []
-     then W
-     else
-       if tl C = []
-       then
-         W(hd C:= i # W (hd C))
-       else
-         W(hd C:= i # W (hd C), hd (tl C):= i # W (hd (tl C)))
-   )\<close>
+type_synonym 'v twl_st_wl_init = \<open>'v twl_st_wl \<times> 'v clauses\<close>
+
+fun get_trail_init_wl :: \<open>'v twl_st_wl_init \<Rightarrow> ('v, nat) ann_lit list\<close> where
+  \<open>get_trail_init_wl ((M, _, _, _, _, _, _), _) = M\<close>
+
+fun get_conflict_init_wl :: \<open>'v twl_st_wl_init \<Rightarrow> 'v cconflict\<close> where
+  \<open>get_conflict_init_wl ((_, _, D, _, _, _, _), _) = D\<close>
+
+fun literals_to_update_init_wl :: \<open>'v twl_st_wl_init \<Rightarrow> 'v clause\<close> where
+  \<open>literals_to_update_init_wl ((_, _, _, _, _, Q, _), _) = Q\<close>
+
+fun other_clauses_init_wl :: \<open>'v twl_st_wl_init \<Rightarrow> 'v clauses\<close> where
+  \<open>other_clauses_init_wl ((_, _, _, _, _, _, _), OC) = OC\<close>
+
+fun add_empty_conflict_init_wl :: \<open>'v twl_st_wl_init \<Rightarrow> 'v twl_st_wl_init\<close> where
+  add_empty_conflict_init_wl_def[simp del]:
+   \<open>add_empty_conflict_init_wl ((M, N, D, NE, UE, Q, W), OC) =
+       ((M, N, Some {#}, NE, UE, {#}, W), add_mset {#} OC)\<close>
+
+fun propagate_unit_init_wl :: \<open>'v literal \<Rightarrow> 'v twl_st_wl_init \<Rightarrow> 'v twl_st_wl_init\<close> where
+  propagate_unit_init_wl_def[simp del]:
+   \<open>propagate_unit_init_wl L ((M, N, D, NE, UE, Q, W), OC) =
+       ((Propagated L 0 # M, N, D, add_mset {#L#} NE, UE, add_mset (-L) Q, W), OC)\<close>
+
+
+fun already_propagated_unit_init_wl :: \<open>'v clause \<Rightarrow> 'v twl_st_wl_init \<Rightarrow> 'v twl_st_wl_init\<close> where
+  already_propagated_unit_init_wl_def[simp del]:
+   \<open>already_propagated_unit_init_wl C ((M, N, D, NE, UE, Q, W), OC) =
+       ((M, N, D, add_mset C NE, UE, Q, W), OC)\<close>
+
+
+fun set_conflict_init_wl :: \<open>'v clause_l \<Rightarrow> 'v twl_st_wl_init \<Rightarrow> 'v twl_st_wl_init\<close> where
+  set_conflict_init_wl_def[simp del]:
+   \<open>set_conflict_init_wl C ((M, N, _, NE, UE, Q, W), OC) =
+       ((M, N, Some (mset C), add_mset (mset C) NE, UE, {#}, W), OC)\<close>
+
+
+fun add_to_clauses_init_wl :: \<open>'v clause_l \<Rightarrow> 'v twl_st_wl_init \<Rightarrow> 'v twl_st_wl_init nres\<close> where
+  add_to_clauses_init_wl_def[simp del]:
+   \<open>add_to_clauses_init_wl C ((M, N, _, NE, UE, Q, W), OC) = do {
+        i \<leftarrow> get_fresh_index N;
+        let W = W((C!0) := W (C!0) @ [i], (C!1) := W (C!1) @ [i]);
+        RETURN ((M, fmupd i (C, True) N, None, NE, UE, Q, W), OC)
+    }\<close>
+
+
+definition init_dt_step_wl :: \<open>'v clause_l \<Rightarrow> 'v twl_st_wl_init \<Rightarrow> 'v twl_st_wl_init nres\<close> where
+  \<open>init_dt_step_wl C S =
+  (case get_conflict_init_wl S of
+    None \<Rightarrow>
+    if length C = 0
+    then RETURN (add_empty_conflict_init_wl S)
+    else if length C = 1
+    then
+      let L = hd C in
+      if undefined_lit (get_trail_init_wl S) L
+      then RETURN (propagate_unit_init_wl L S)
+      else if L \<in> lits_of_l (get_trail_init_wl S)
+      then RETURN (already_propagated_unit_init_wl (mset C) S)
+      else RETURN (set_conflict_init_wl C S)
+    else
+        add_to_clauses_init_wl C S
+  | Some D \<Rightarrow>
+      RETURN (add_to_other_init C S))\<close>
+
+definition init_dt_wl :: \<open>'v clause_l list \<Rightarrow> 'v twl_st_wl_init \<Rightarrow> 'v twl_st_wl_init nres\<close> where
+  \<open>init_dt_wl CS = nfoldli CS (\<lambda>_. True) init_dt_step_wl\<close>
+
+definition state_wl_l_init :: \<open>('v twl_st_wl_init \<times> 'v twl_st_l_init) set\<close> where
+  \<open>state_wl_l_init = {(S, S'). (fst S, fst S') \<in> state_wl_l None \<and>
+      other_clauses_init_wl S = other_clauses_l_init S'}\<close>
+
+fun correct_watching_init :: \<open>'v twl_st_wl_init \<Rightarrow> bool\<close> where
+  [simp del]: \<open>correct_watching_init ((M, N, D, NE, UE, Q, W), _) \<longleftrightarrow>
+    ((\<forall>L. mset (W L) = clause_to_update L (M, N, D, NE, UE, {#}, {#})))\<close>
+
+named_theorems twl_st_wl_init
+
+lemma [twl_st_wl_init]:
+  assumes \<open>(S, S') \<in> state_wl_l_init\<close>
+  shows
+    \<open>get_conflict_l_init S' = get_conflict_init_wl S\<close>
+    \<open>get_trail_l_init S' = get_trail_init_wl S\<close>
+  using assms
+  by (cases S; cases S'; auto simp: state_wl_l_init_def state_wl_l_def)+
+
 
 lemma image_mset_Suc: \<open>Suc `# {#C \<in># M. P C#} = {#C \<in># Suc `# M. P (C-1)#}\<close>
   by (induction M) auto
 
-lemma clause_to_update_def2:
-  \<open>clause_to_update L (M, C # N, U, D, NE, UE, {#}, {#}) =
-    image_mset Suc (filter_mset
-      (\<lambda>C::nat. L \<in> set (watched_l (N!C)))
-      (mset [0..<length N]))\<close>
-proof -
-  have 1: \<open>Suc `# mset [0..<length N] =  mset [1..<Suc (length N)]\<close>
-    unfolding mset_map[symmetric]
-    using map_add_upt[of 1 \<open>length N\<close>] by force
-  show ?thesis
-    unfolding clause_to_update_def image_mset_Suc 1 get_clauses_l.simps length_Cons
-    by (rule filter_mset_cong) (auto split: if_splits)
-qed
+lemma correct_watching_init_add_unit:
+  \<open>correct_watching_init ((M, N, D, add_mset C NE, UE, Q, W), OC) \<longleftrightarrow>
+         correct_watching_init ((M, N, D, NE, UE, Q, W), OC)\<close>
+  unfolding correct_watching_init.simps clause_to_update_def Ball_def
+  by (auto simp: correct_watching.simps all_lits_of_mm_add_mset
+      all_lits_of_m_add_mset Ball_def all_conj_distrib clause_to_update_def)
 
-lemma clause_to_update_Cons: \<open>clause_to_update L (M, C # C' # N, U, D, NE, UE, {#}, {#}) =
-         (if L \<in> set (watched_l C') then {#1#} else {#}) +
-         Suc `# clause_to_update L (M, C # N, U, D, NE, UE, {#}, {#})\<close> for L C
-proof -
-  define dont_be_silly where
-    \<open>dont_be_silly L = {#C \<in># mset [0..<length N]. L \<in> set (watched_l (N ! C))#}\<close> for L
-  have [simp]: \<open>Suc `# mset_set {a..<b} = mset_set {Suc a..<Suc b}\<close> for a b
-    by (simp add: image_mset_mset_set)
-  have 1: \<open>mset [0..<Suc (length N)] = add_mset 0 (mset [1..<Suc (length N)])\<close>
-    by (subst upt_conv_Cons) auto
-  have 2: \<open>{#C \<in># mset [1..<Suc (length N)].
-            L \<in> set (watched_l ((C' # N) ! C))#} = Suc `# {#C \<in># mset [0..<length N].
-            L \<in> set (watched_l (N ! C))#}\<close> for L
-    unfolding image_mset_Suc
-    by (rule filter_mset_cong_inner_outer) (auto split: if_splits simp: atLeastLessThanSuc)
-  show ?thesis
-    unfolding clause_to_update_def2 length_Cons mset.simps filter_mset_add_mset 1
-    unfolding dont_be_silly_def[symmetric] 2
-    by auto
-qed
+lemma correct_watching_init_propagate:
+  \<open>correct_watching_init ((L # M, N, D, NE, UE, Q, W), OC) \<longleftrightarrow>
+         correct_watching_init ((M, N, D, NE, UE, Q, W), OC)\<close>
+  \<open>correct_watching_init ((M, N, D, NE, UE, add_mset C Q, W), OC) \<longleftrightarrow>
+         correct_watching_init ((M, N, D, NE, UE, Q, W), OC)\<close>
+  unfolding correct_watching_init.simps clause_to_update_def Ball_def
+  by (auto simp: correct_watching.simps all_lits_of_mm_add_mset
+      all_lits_of_m_add_mset Ball_def all_conj_distrib clause_to_update_def)
 
-lemma calculate_correct_watching:
-   \<open>mset ((calculate_correct_watching N (\<lambda>_. []) i) L) =
-           image_mset (\<lambda>n. n+i-1) (clause_to_update L (M, C # N, U, D, NE, UE, {#}, {#}))\<close>
+
+lemma init_dt_step_wl_init_dt_step:
+  assumes S_S': \<open>(S, S') \<in> state_wl_l_init\<close> and corr: \<open>correct_watching_init S\<close>
+  shows \<open>init_dt_step_wl C S \<le> \<Down> {(S, S'). (S, S') \<in> state_wl_l_init \<and> correct_watching_init S}
+          (init_dt_step C S')\<close>
+   (is \<open>_ \<le> \<Down> ?A _\<close>)
 proof -
-  show ?thesis
-  proof (induction N arbitrary: i L)
-    case Nil
-    then show ?case by (auto simp: clause_to_update_def)
-  next
-    case (Cons C N)
-    consider
-      (Nil) \<open>C = []\<close> |
-      (C1) K where \<open>C = [K]\<close> |
-      (C2) K K' C' where \<open>C = K # K' # C'\<close>
-      by (cases C; cases \<open>tl C\<close>) auto
-    then show ?case
-    proof cases
-      case Nil note C = this
-      show ?thesis
-        using Cons C
-        by (simp add: clause_to_update_Cons Let_def)
-    next
-      case C1 note C = this
-      show ?thesis
-        by (auto simp add: C Let_def Cons clause_to_update_Cons)
-    next
-      case C2
-      then show ?thesis
-        using Cons by (simp add: clause_to_update_Cons Let_def)
-    qed
+  have confl: \<open>(get_conflict_init_wl S, get_conflict_l_init S') \<in> \<langle>Id\<rangle>option_rel\<close>
+    using S_S' by (auto simp: twl_st_wl_init)
+  have false: \<open>(add_empty_conflict_init_wl S, add_empty_conflict_init_l S') \<in> ?A\<close>
+    using S_S' corr
+    apply (cases S; cases S')
+    apply (auto simp: add_empty_conflict_init_wl_def add_empty_conflict_init_l_def
+        correct_watching_init.simps
+        state_wl_l_init_def state_wl_l_def correct_watching.simps clause_to_update_def)
+    done
+  have propa_unit:
+    \<open>(propagate_unit_init_wl (hd C) S, propagate_unit_init_l (hd C) S') \<in> ?A\<close>
+
+    using S_S' corr apply (cases S; cases S')
+    apply (auto simp: propagate_unit_init_l_def propagate_unit_init_wl_def
+        state_wl_l_init_def state_wl_l_def correct_watching_init.simps clause_to_update_def
+        all_lits_of_mm_add_mset all_lits_of_m_add_mset all_lits_of_mm_union)
+    done
+  have already_propa:
+    \<open>(already_propagated_unit_init_wl (mset C) S, already_propagated_unit_init_l (mset C) S') \<in> ?A\<close>
+    using S_S' corr
+    by (cases S; cases S')
+       (auto simp: already_propagated_unit_init_wl_def already_propagated_unit_init_l_def
+        state_wl_l_init_def state_wl_l_def correct_watching.simps clause_to_update_def
+        all_lits_of_mm_add_mset all_lits_of_m_add_mset correct_watching_init.simps)
+  have set_conflict: \<open>(set_conflict_init_wl C S, set_conflict_init_l C S') \<in> ?A\<close>
+    using S_S' corr
+    by (cases S; cases S')
+       (auto simp: set_conflict_init_wl_def set_conflict_init_l_def
+        state_wl_l_init_def state_wl_l_def correct_watching.simps clause_to_update_def
+        all_lits_of_mm_add_mset all_lits_of_m_add_mset correct_watching_init.simps)
+  have add_to_clauses_init_wl: \<open>add_to_clauses_init_wl C S
+          \<le> \<Down> {(S, S'). (S, S') \<in> state_wl_l_init \<and> correct_watching_init S}
+               (add_to_clauses_init_l C S')\<close>
+    if C: \<open>length C \<ge> 2\<close>
+  proof -
+    have [iff]: \<open>C ! Suc 0 \<notin> set (watched_l C) \<longleftrightarrow> False\<close>
+      \<open>C ! 0 \<notin> set (watched_l C) \<longleftrightarrow> False\<close> and
+      [dest!]: \<open>\<And>L. L \<noteq> C ! 0 \<Longrightarrow> L \<noteq> C ! Suc 0 \<Longrightarrow> L \<in> set (watched_l C) \<Longrightarrow> False\<close>
+      using C by (cases C; cases \<open>tl C\<close>; auto)+
+    show ?thesis
+      using S_S' corr
+      by (cases S; cases S')
+        (auto 5 5 simp: add_to_clauses_init_wl_def add_to_clauses_init_l_def get_fresh_index_def
+          state_wl_l_init_def state_wl_l_def correct_watching.simps clause_to_update_def
+          all_lits_of_mm_add_mset all_lits_of_m_add_mset correct_watching_init.simps
+          RES_RETURN_RES
+          intro!: RES_refine filter_mset_cong2)
   qed
+  have add_to_other_init:
+    \<open>(add_to_other_init C S, add_to_other_init C S') \<in> ?A\<close>
+    using S_S' corr
+    by (cases S; cases S')
+       (auto simp: state_wl_l_init_def state_wl_l_def correct_watching.simps clause_to_update_def
+        all_lits_of_mm_add_mset all_lits_of_m_add_mset correct_watching_init.simps)
+  show ?thesis
+    unfolding init_dt_step_wl_def init_dt_step_def
+    apply (refine_vcg confl false propa_unit already_propa set_conflict
+        add_to_clauses_init_wl add_to_other_init)
+    subgoal by simp
+    subgoal by simp
+    subgoal using S_S' by (simp add: twl_st_wl_init)
+    subgoal using S_S' by (simp add: twl_st_wl_init)
+    subgoal by linarith
+    done
 qed
 
-lemma twl_struct_invs_init_twl_struct_invs:
-  \<open>snd S = {#} \<Longrightarrow> twl_struct_invs_init S \<longleftrightarrow> twl_struct_invs (fst S)\<close>
-  by (cases S) (auto simp: twl_struct_invs_def twl_struct_invs_init_def)
+lemma init_dt_wl_init_dt:
+  assumes S_S': \<open>(S, S') \<in> state_wl_l_init\<close> and corr: \<open>correct_watching_init S\<close>
+  shows \<open>init_dt_wl C S \<le> \<Down> {(S, S'). (S, S') \<in> state_wl_l_init \<and> correct_watching_init S}
+          (init_dt C S')\<close>
+proof -
+  have C: \<open>(C, C) \<in> \<langle>Id\<rangle>list_rel\<close>
+    by simp
+  show ?thesis
+    unfolding init_dt_wl_def init_dt_def
+    apply (refine_vcg C S_S' )
+    subgoal using S_S' corr by fast
+    subgoal by simp
+    subgoal by (auto intro!: init_dt_step_wl_init_dt_step)
+    done
+qed
 
 (* TODO Kill?
 
